wip

libcrux-intrinsics/src/avx2_extract.rs
@@ -6,12 +6,12 @@
 #[cfg(hax)]
 #[derive(Clone, Copy)]
 #[hax_lib::opaque_type]
-#[hax_lib::fstar::after(interface, "val vec256_as_i16x16 (x:$:{Vec256}) : t_Array i16 (sz 16)")]
+#[hax_lib::fstar::replace(interface, "unfold type $:{Vec256} = bit_vec 256")]
 pub struct Vec256(u8);
 
 #[cfg(hax)]
 #[derive(Copy, Clone)]
-#[hax_lib::fstar::after(interface, "val vec128_as_i16x8 (x:$:{Vec128}) : t_Array i16 (sz 8)")]
+#[hax_lib::fstar::replace(interface, "unfold type $:{Vec128} = bit_vec 128")]
 #[hax_lib::opaque_type]
 pub struct Vec128(u8);
 
@@ -19,18 +19,6 @@ pub struct Vec128(u8);
 pub type Vec256 = u8;
 #[cfg(not(hax))]
 pub type Vec128 = u8;
-
-#[hax_lib::fstar::replace(interface, "unfold type $:{BitVector256} = bit_vec 256")]
-pub struct BitVector256;
-#[hax_lib::fstar::replace(interface, "unfold type $:{BitVector128} = bit_vec 128")]
-pub struct BitVector128;
-
-pub fn bv256(vec: Vec256) -> BitVector256 {
-    unimplemented!()
-}
-pub fn bv128(vec: Vec128) -> BitVector128 {
-    unimplemented!()
-}
 
 pub fn mm256_storeu_si256_i16(output: &mut [i16], vector: Vec256) {
     debug_assert_eq!(output.len(), 16);
@@ -251,6 +239,10 @@ pub fn mm256_srli_epi64<const SHIFT_BY: i32>(vector: Vec256) -> Vec256 {
     unimplemented!()
 }
 
+#[hax_lib::fstar::replace(
+    interface,
+    "unfold let ${mm256_slli_epi16::<0>} = BitVec.Intrinsics.mm256_slli_epi16"
+)]
 pub fn mm256_slli_epi16<const SHIFT_BY: i32>(vector: Vec256) -> Vec256 {
     debug_assert!(SHIFT_BY >= 0 && SHIFT_BY < 16);
     unimplemented!()
@@ -289,6 +281,10 @@ pub fn mm256_unpackhi_epi32(lhs: Vec256, rhs: Vec256) -> Vec256 {
     unimplemented!()
 }
 
+#[hax_lib::fstar::replace(
+    interface,
+    "unfold let ${mm256_castsi256_si128} = BitVec.Intrinsics.mm256_castsi256_si128"
+)]
 pub fn mm256_castsi256_si128(vector: Vec256) -> Vec128 {
     unimplemented!()
 }
@@ -300,6 +296,10 @@ pub fn mm256_cvtepi16_epi32(vector: Vec128) -> Vec256 {
     unimplemented!()
 }
 
+#[hax_lib::fstar::replace(
+    interface,
+    "unfold let ${mm_packs_epi16} = BitVec.Intrinsics.mm_packs_epi16"
+)]
 pub fn mm_packs_epi16(lhs: Vec128, rhs: Vec128) -> Vec128 {
     unimplemented!()
 }
@@ -307,6 +307,10 @@ pub fn mm256_packs_epi32(lhs: Vec256, rhs: Vec256) -> Vec256 {
     unimplemented!()
 }
 
+#[hax_lib::fstar::replace(
+    interface,
+    "unfold let ${mm256_extracti128_si256::<0>} = BitVec.Intrinsics.mm256_extracti128_si256"
+)]
 pub fn mm256_extracti128_si256<const CONTROL: i32>(vector: Vec256) -> Vec128 {
     debug_assert!(CONTROL == 0 || CONTROL == 1);
     unimplemented!()
@@ -322,6 +326,10 @@ pub fn mm256_blend_epi16<const CONTROL: i32>(lhs: Vec256, rhs: Vec256) -> Vec256
     unimplemented!()
 }
 
+#[hax_lib::fstar::replace(
+    interface,
+    "unfold let ${mm_movemask_epi8} = BitVec.Intrinsics.mm_movemask_epi8"
+)]
 pub fn mm_movemask_epi8(vector: Vec128) -> i32 {
     unimplemented!()
 }
